Updated assumptions necessary for the example to work

examples/lowstar_permissions/Test.Array.fst
@@ -52,14 +52,13 @@ let read_write_without_sharing () : RST.RST unit
   A.free b;
   ()
 
-#set-options "--warn_error '-271-296'"
+#set-options "--warn_error '-271-296' --z3rlimit 60"
 let read_write_with_sharing () : RST.RST unit
   (R.empty_resource)
   (fun _ -> R.empty_resource)
   (fun _ -> True)
   (fun _ _ _ -> True)
   =
-  admit();
   let b = A.alloc 2ul 42ul in
   let x1 = A.index b 0ul in
   A.upd b 0ul FStar.UInt32.(x1 +%^ 1ul);
@@ -77,24 +76,21 @@ let read_write_with_sharing () : RST.RST unit
     (fun p -> R.(A.array_resource (fst p) <*> A.array_resource (snd p) <*> A.array_resource b1))
     (let f = fun _ -> A.split #FStar.UInt32.t b 1ul in f) //TODO: remove let binding
   in
-  let h = HST.get () in
-   let full = R.(A.array_resource b_first <*> A.array_resource b_second <*> A.array_resource b1) in
-  let delta = R.(A.array_resource b_first <*> A.array_resource b1) in
-//  assume(R.inv full h ==> R.inv delta h);
   let x2 = RST.rst_frame
     (R.(A.array_resource b_first <*> A.array_resource b_second <*> A.array_resource b1))
     (fun _ -> (R.(A.array_resource b_first <*> A.array_resource b_second <*> A.array_resource b1)))
     (fun _ -> A.index b_second 0ul)
   in
-  let h' = HST.get () in
-  // assume(R.sel (R.view_of delta) h == R.sel (R.view_of delta) h' ==>
-  //   R.sel (A.array_view b_first ) h == R.sel (A.array_view b_first) h' /\
-  //   R.sel (A.array_view b1 ) h == R.sel (A.array_view b1) h');
+  let sel = RST.get R.(A.array_resource b_first <*> A.array_resource b_second <*> A.array_resource b1) in
+  assume(A.get_perm b_first sel == A.get_perm b_second sel);
   RST.rst_frame
     (R.(A.array_resource b_first <*> A.array_resource b_second <*> A.array_resource b1))
     (fun _ -> R.(A.array_resource b <*> A.array_resource b1))
     (fun _ -> A.glue b b_first b_second);
 
-  let h'' = HST.get () in
+  let sel = RST.get R.(A.array_resource b <*> A.array_resource b1) in
+  assume(A.summable_permissions b b1 sel);
   A.gather b b1;
+  let sel = RST.get R.(A.array_resource b) in
+  assume(P.allows_write (A.get_perm b sel));
   A.free b
